Foundation/Modal/Kripke/SimpleExtension.lean
@@ -3,87 +3,91 @@ import Mathlib.Data.Finite.Sum
 
 namespace LO.Modal.Kripke
 
-def FiniteTransitiveTree.SimpleExtension (F : FiniteTransitiveTree) : Kripke.FiniteTransitiveTree where
+def Frame.extendRoot (F : Kripke.Frame) (r : F.World) [F.IsRooted r] : Kripke.Frame where
   World := Unit ⊕ F.World
   Rel x y :=
     match x, y with
     | .inr x, .inr y => x ≺ y
     | .inl _, .inr _ => True
     | _ , _ => False
-  root := .inl ()
-  root_rooted := by
-    intro w;
-    match w with
-    | .inl _ => simp;
-    | .inr x => simp [Frame.Rel]
-  rel_assymetric := by
-    intro x y hxy;
-    match x, y with
-    | .inl x, _ => simp;
-    | .inr x, .inr y => exact F.rel_assymetric hxy;
-  rel_transitive := by
-    intro x y z hxy hyz;
-    match x, y, z with
-    | .inl _, .inr _, .inr _ => simp;
-    | .inr x, .inr y, .inr z => exact F.rel_transitive hxy hyz;
-postfix:max "↧" => FiniteTransitiveTree.SimpleExtension
 
+namespace Frame.extendRoot
 
-namespace FiniteTransitiveTree.SimpleExtension
+variable {F : Frame} {r : F.World} [F.IsRooted r] {x y : F.World}
 
-variable {T : FiniteTransitiveTree} {x y : T.World}
+instance [f : F.IsFinite] : (F.extendRoot r).IsFinite := by
+  unfold Frame.extendRoot;
+  apply Frame.isFinite_iff _ |>.mpr;
+  infer_instance;
 
-instance : Coe (T.World) (T↧.World) := ⟨Sum.inr⟩
+protected abbrev root : (F.extendRoot r).World := .inl ()
 
-@[simp] lemma root_not_original : (Sum.inr x) ≠ T↧.root := by simp [SimpleExtension]
+instance instIsRooted : (F.extendRoot r).IsRooted extendRoot.root where
+  root_generates := by
+    intro x h;
+    match x with
+    | .inl _ => contradiction;
+    | .inr x => apply Relation.TransGen.single; tauto;
 
-lemma root_eq : (Sum.inl ()) = T↧.root := by simp [SimpleExtension];
+lemma rel_assymetric (F_assym : Assymetric F) : Assymetric (F.extendRoot r).Rel := by
+  intro x y hxy;
+  match x, y with
+  | .inl x, _ => simp_all [Frame.extendRoot]
+  | .inr x, .inr y => exact F_assym hxy;
 
-lemma forth (h : x ≺ y) : T↧.Rel x y := by simpa [SimpleExtension];
+lemma rel_transitive (F_trans : Transitive F) : Transitive (F.extendRoot r).Rel := by
+  intro x y z hxy hyz;
+  match x, y, z with
+  | .inl _, .inr _, .inr _ => simp_all [Frame.extendRoot]
+  | .inr x, .inr y, .inr z => exact F_trans hxy hyz;
 
-def p_morphism : T.toFrame →ₚ (T↧.toFrame) where
-  toFun x := x
-  forth := forth
+instance {r : F.World} [tree : F.IsTree r] : (F.extendRoot r).IsTree extendRoot.root where
+  rel_assymetric := rel_assymetric $ tree.rel_assymetric;
+  rel_transitive := rel_transitive $ tree.rel_transitive
+
+instance [F.IsFiniteTree r] : (F.extendRoot r).IsFiniteTree (extendRoot.root) where
+
+def pMorphism : F →ₚ (F.extendRoot r) where
+  toFun := Sum.inr
+  forth := by simp [Frame.extendRoot];
   back {x y} h := by
     match y with
-    | .inl r => simp [Frame.Rel', SimpleExtension] at h;
+    | .inl r => simp [Frame.Rel', Frame.extendRoot] at h;
     | .inr y => use y; simpa using h;
 
-lemma through_original_root {x : T↧.World} (h : T↧.root ≺ x) : x = T.root ∨ (Sum.inr T.root ≺ x) := by
+lemma through_original_root [F.IsTree r] {x : (F.extendRoot r).World} (h : extendRoot.root ≺ x) : x = extendRoot.root ∨ (Sum.inr r ≺^+ x) := by
   match x with
-  | .inl x =>
-    have := T↧.rel_irreflexive _ h;
-    contradiction;
+  | .inl x => simp;
   | .inr x =>
-    by_cases h : x = T.root;
-    . subst h; left; tauto;
-    . right; exact FiniteTransitiveTree.SimpleExtension.forth $ T.root_rooted x h;
+    by_cases e : x = r;
+    . subst e;
+      sorry;
+    . right;
+      apply Relation.TransGen.single;
+      apply pMorphism (F := F).forth;
+      sorry;
 
-end FiniteTransitiveTree.SimpleExtension
+end Frame.extendRoot
 
 
-abbrev FiniteTransitiveTreeModel.SimpleExtension (M : FiniteTransitiveTreeModel) : Kripke.FiniteTransitiveTreeModel where
-  toFiniteTransitiveTree := M.toFiniteTransitiveTree↧
+abbrev Model.extendRoot (M : Kripke.Model) (r : M.World) [M.IsRooted r] : Kripke.Model where
+  toFrame := M.toFrame.extendRoot r
   Val x a :=
     match x with
-    | .inl _ => M.Val M.root a
+    | .inl _ => M.Val r a
     | .inr x => M.Val x a
-postfix:max "↧" => FiniteTransitiveTreeModel.SimpleExtension
 
+namespace Model.extendRoot
 
-namespace FiniteTransitiveTreeModel.SimpleExtension
+variable {M : Model} {r : M.World} [M.IsRooted r] {x y : M.World}
 
-variable {M : FiniteTransitiveTreeModel}
+def pMorphism : Model.PseudoEpimorphism M (M.extendRoot r) := Model.PseudoEpimorphism.ofAtomic (@Frame.extendRoot.pMorphism M.toFrame r inferInstance) $ by
+  intros; rfl;
 
-instance : Coe (M.World) (M↧.World) := ⟨Sum.inr⟩
+lemma modal_equivalence_original_world {x : M.World} : ModalEquivalent (M₁ := M) (M₂ := M.extendRoot r) x (Sum.inr x) := by
+  apply Model.PseudoEpimorphism.modal_equivalence pMorphism;
 
-def p_morphism : M.toModel →ₚ (M↧.toModel) := Model.PseudoEpimorphism.ofAtomic (FiniteTransitiveTree.SimpleExtension.p_morphism) $ by
-  simp [FiniteTransitiveTree.SimpleExtension.p_morphism];
-
-lemma modal_equivalence_original_world {x : M.toModel.World} : ModalEquivalent (M₁ := M.toModel) (M₂ := (M↧).toModel) x (Sum.inr x) := by
-  apply Model.PseudoEpimorphism.modal_equivalence p_morphism;
-
-end FiniteTransitiveTreeModel.SimpleExtension
+end Model.extendRoot
 
 
 end LO.Modal.Kripke
