Foundation/Modal/Kripke/Tree.lean
@@ -6,55 +6,45 @@ namespace LO.Modal
 namespace Kripke
 
 
-class Frame.IsTree (F : Kripke.Frame) extends F.IsRooted where
-  rel_assymetric : Assymetric F.Rel
-  rel_transitive : Transitive F.Rel
+class Frame.IsTree (F : Kripke.Frame) (root : F.World) extends F.IsRooted root where
+  protected rel_assymetric : Assymetric F.Rel
+  protected rel_transitive : Transitive F.Rel
 
 namespace Frame.IsTree
 
-variable {F : Frame} [F.IsTree]
+variable {F : Frame} {r : F.World}
 
-lemma rel_irreflexive : Irreflexive F.Rel := irreflexive_of_assymetric $ IsTree.rel_assymetric
+protected lemma rel_irreflexive [F.IsTree r] : Irreflexive F.Rel := irreflexive_of_assymetric (IsTree.rel_assymetric r)
 
 end Frame.IsTree
 
-
-class Frame.IsFiniteTree (F : Kripke.Frame) extends F.IsFinite, F.IsTree where
-
-
-class Model.IsTree (M : Kripke.Model) where
-  [frame_is_tree : M.toFrame.IsTree]
-
-class Model.IsFiniteTree (M : Kripke.Model) where
-  [frame_is_finite_tree : M.toFrame.IsFiniteTree]
+class Frame.IsFiniteTree (F : Kripke.Frame) (r : F.World) extends F.IsFinite, F.IsTree r where
 
 
 
 section TreeUnravelling
 
-variable {F : Frame} {r : F.World}
+variable {F : Kripke.Frame} {r : F.World}
 
 def Frame.mkTreeUnravelling (F : Frame) (r : F.World) : Kripke.Frame where
   World := { c : List F.World // [r] <+: c ∧ c.Chain' F.Rel }
   Rel cx cy := ∃ z, cy.1 = cx.1 ++ [z]
   world_nonempty := ⟨[r], (by simp)⟩
 
-infix:100 "🌲" => Frame.mkTreeUnravelling
-
 namespace Frame.treeUnravelling
 
 @[simp]
-lemma not_nil {c : (F🌲r).World} : c.1 ≠ [] := by
+lemma not_nil {c : (F.mkTreeUnravelling r).World} : c.1 ≠ [] := by
   have := c.2.1;
   by_contra;
   simp_all;
 
-lemma rel_length {x y : (F🌲r).World} (h : x ≺ y) : x.1.length < y.1.length := by
+lemma rel_length {x y : (F.mkTreeUnravelling r).World} (h : x ≺ y) : x.1.length < y.1.length := by
   obtain ⟨z, hz⟩ := h;
   simp_all;
 
 
-lemma transrel_def {cx cy : (F🌲r).World} : cx ≺^+ cy ↔ ∃ l ≠ [], cy.1 = cx.1 ++ l ∧ (List.Chain' F.Rel (cx.1.head (by simp) :: l)) := by
+lemma transrel_def {cx cy : (F.mkTreeUnravelling r).World} : cx ≺^+ cy ↔ ∃ l ≠ [], cy.1 = cx.1 ++ l ∧ (List.Chain' F.Rel (cx.1.head (by simp) :: l)) := by
   constructor;
   . intro h;
     induction h using Relation.TransGen.head_induction_on with
@@ -90,17 +80,17 @@ lemma transrel_def {cx cy : (F🌲r).World} : cx ≺^+ cy ↔ ∃ l ≠ [], cy.1
       . sorry;
       . sorry;
 
-protected lemma rel_irreflexive : Irreflexive (F🌲r).Rel := by
+protected lemma rel_irreflexive : Irreflexive (F.mkTreeUnravelling r).Rel := by
   intro x; simp [Frame.mkTreeUnravelling];
 
-protected lemma rel_assymetric : Assymetric (F🌲r).Rel := by
+protected lemma rel_assymetric : Assymetric (F.mkTreeUnravelling r).Rel := by
   rintro x y hxy;
   by_contra hyx;
   replace hxy := rel_length hxy;
   replace hyx := rel_length hyx;
   exact hxy.not_lt hyx;
 
-protected def pMorphism (F : Frame) (r : F) : F🌲r →ₚ F where
+protected def pMorphism (F : Frame) (r : F) : F.mkTreeUnravelling r →ₚ F where
   toFun c := c.1.getLast (by simp)
   forth {cx cy} h := by
     obtain ⟨z, hz⟩ := h;
@@ -126,9 +116,9 @@ protected def pMorphism (F : Frame) (r : F) : F🌲r →ₚ F where
           convert h;
           exact List.mem_getLast?_eq_getLast hz |>.2;
 
+protected abbrev root : (F.mkTreeUnravelling r).World := ⟨[r], by tauto⟩
 
-instance : (F🌲r).IsRooted where
-  root := ⟨[r], by tauto⟩
+instance : (F.mkTreeUnravelling r).IsRooted treeUnravelling.root where
   root_generates := by
     rintro ⟨_, ⟨l, rfl⟩, l_chain⟩ hn;
     apply transrel_def.mpr;
@@ -137,33 +127,32 @@ instance : (F🌲r).IsRooted where
 end Frame.treeUnravelling
 
 
-abbrev Frame.mkTransTreeUnravelling (F : Frame) (r : F.World) := (F🌲r)^+
-infix:100 "🌲^+" => Frame.mkTransTreeUnravelling
+abbrev Frame.mkTransTreeUnravelling (F : Frame) (r : F.World) := (F.mkTreeUnravelling r)^+
 
 
-namespace Frame.transTreeUnravelling
+namespace Frame.mkTransTreeUnravelling
 
 @[simp]
-lemma not_nil {c : (F🌲^+r).World} : c.1 ≠ [] := by
+lemma not_nil {c : (F.mkTransTreeUnravelling r).World} : c.1 ≠ [] := by
   by_contra;
   have := c.2.1;
   simp_all;
 
-lemma rel_length {x y : (F🌲^+r).World} (Rxy : x ≺ y) : x.1.length < y.1.length := by
+lemma rel_length {x y : (F.mkTransTreeUnravelling r).World} (Rxy : x ≺ y) : x.1.length < y.1.length := by
   induction Rxy with
   | single Rxy => exact treeUnravelling.rel_length Rxy;
   | tail _ h ih => have := treeUnravelling.rel_length h; omega;
 
-protected lemma rel_transitive : Transitive (F🌲^+r) := Frame.RelTransGen.transitive
+protected lemma rel_transitive : Transitive (F.mkTransTreeUnravelling r) := Frame.RelTransGen.transitive
 
-protected lemma rel_asymmetric : Assymetric (F🌲^+r) := by
+protected lemma rel_asymmetric : Assymetric (F.mkTransTreeUnravelling r) := by
   rintro x y hxy;
   by_contra hyx;
   replace hxy := rel_length hxy;
   replace hyx := rel_length hyx;
   exact hxy.not_lt hyx;
 
-lemma rel_def {x y : (F🌲^+r).World} : x ≺ y ↔ (x.1.length < y.1.length ∧ x.1 <+: y.1) := by
+lemma rel_def {x y : (F.mkTransTreeUnravelling r).World} : x ≺ y ↔ (x.1.length < y.1.length ∧ x.1 <+: y.1) := by
   constructor;
   . intro Rxy;
     induction Rxy with
@@ -205,49 +194,72 @@ lemma rel_def {x y : (F🌲^+r).World} : x ≺ y ↔ (x.1.length < y.1.length �
       . simp_all;
 
 
-abbrev pMorphism (F : Frame) (F_trans : Transitive F.Rel) (r : F) : (F🌲^+r) →ₚ F := (treeUnravelling.pMorphism F r).TransitiveClosure F_trans
+abbrev pMorphism (F : Frame) (F_trans : Transitive F.Rel) (r : F) : (F.mkTransTreeUnravelling r) →ₚ F := (treeUnravelling.pMorphism F r).TransitiveClosure F_trans
 
-instance : (F🌲^+r).IsRooted := inferInstance
+protected abbrev root : (F.mkTransTreeUnravelling r).World := treeUnravelling.root
 
-instance {F : Frame} [DecidableEq F.World] [F.IsFinite] {r : F.World}
-  (F_trans : Transitive F) (F_irrefl : Irreflexive F)
-  : ((F↾r)🌲^+ ⟨r, by tauto⟩).IsFiniteTree where
-  rel_transitive := Frame.transTreeUnravelling.rel_transitive
-  rel_assymetric := Frame.transTreeUnravelling.rel_asymmetric
+instance instIsRooted : (F.mkTransTreeUnravelling r).IsRooted (mkTransTreeUnravelling.root) := inferInstance
+
+instance instIsTree {F : Frame} [DecidableEq F.World] [F.IsFinite] {r : F.World} (F_trans : Transitive F) (F_irrefl : Irreflexive F)
+  : (F.mkTransTreeUnravelling r).IsFiniteTree (mkTransTreeUnravelling.root) where
+  root_generates := by
+    intro w;
+    exact Frame.mkTransTreeUnravelling.instIsRooted.root_generates w;
+  rel_transitive := mkTransTreeUnravelling.rel_transitive
+  rel_assymetric := mkTransTreeUnravelling.rel_asymmetric
   world_finite := by
-    suffices h : Finite { x // List.Chain' (F.pointGenerate r).Rel x } by
-     exact
+    suffices h : Finite { x // List.Chain' F.Rel x } by
+      exact
        Finite.of_injective
-       (β := { x // List.Chain' (F.pointGenerate r).Rel x })
+       (β := { x // List.Chain' F.Rel x })
        (fun x => ⟨x.1, x.2.2⟩)
        (by rintro ⟨x, hx⟩ ⟨y, hy⟩; simp_all);
-    apply List.chains_finite
-      (Frame.pointGenerate.rel_trans (r := r) F_trans)
-      (Frame.pointGenerate.rel_irrefl (r := r) F_irrefl);
+    apply List.chains_finite F_trans F_irrefl;
 
-end Frame.transTreeUnravelling
+end Frame.mkTransTreeUnravelling
 
 
-def Model.mkTreeUnravelling (M : Kripke.Model) (r : M.World) : Kripke.Model where
-  toFrame := M.toFrame🌲r
-  Val c a := M.Val (c.1.getLast (by simp)) a
-infix:100 "🌲" => Model.mkTreeUnravelling
+instance {F : Frame} [DecidableEq F.World] [F.IsFinite] {r : F.World} (F_trans : Transitive F) (F_irrefl : Irreflexive F)
+  : ((F↾r).mkTransTreeUnravelling Frame.pointGenerate.root).IsFiniteTree (Frame.mkTransTreeUnravelling.root) :=
+    Frame.mkTransTreeUnravelling.instIsTree
+    (Frame.pointGenerate.rel_trans F_trans)
+    (Frame.pointGenerate.rel_irrefl F_irrefl)
 
-def Model.mkTreeUnravelling.pMorphism (M : Kripke.Model) (r : M.World) : (M🌲r) →ₚ M :=
+
+def Model.mkTreeUnravelling (M : Kripke.Model) (r : M.World) : Kripke.Model := ⟨M.toFrame.mkTreeUnravelling r, λ c a => M.Val (c.1.getLast (by simp)) a⟩
+
+def Model.mkTreeUnravelling.pMorphism (M : Kripke.Model) (r : M.World) : (M.mkTreeUnravelling r) →ₚ M :=
   PseudoEpimorphism.ofAtomic (Frame.treeUnravelling.pMorphism M.toFrame r) $ by rfl;
 
 
-def Model.mkTransTreeUnravelling (M : Kripke.Model) (r : M.World) : Kripke.Model where
-  toFrame := M.toFrame🌲^+r
-  Val c a := M.Val (c.1.getLast (by simp)) a
-infix:100 "🌲^+" => Model.mkTransTreeUnravelling
+def Model.mkTransTreeUnravelling (M : Kripke.Model) (r : M.World) : Kripke.Model := ⟨M.toFrame.mkTransTreeUnravelling r, λ c a => M.Val (c.1.getLast (by simp)) a⟩
 
-def Model.mkTransTreeUnravelling.pMorphism (M : Kripke.Model) (M_trans : Transitive M.Rel) (r : M.World) : M🌲^+r →ₚ M :=
-  PseudoEpimorphism.ofAtomic (Frame.transTreeUnravelling.pMorphism M.toFrame M_trans r) $ by rfl;
+namespace Model.mkTransTreeUnravelling
 
-lemma Model.mkTransTreeUnravelling.modal_equivalence_at_root (M : Kripke.Model) (M_trans : Transitive M.Rel) (r : M.World)
-  : ModalEquivalent (M₁ := M🌲^+r) (M₂ := M) ⟨[r], by simp⟩ r
-  := Model.PseudoEpimorphism.modal_equivalence (Model.mkTransTreeUnravelling.pMorphism M M_trans r) (⟨[r], by simp⟩)
+protected def pMorphism (M : Kripke.Model) (M_trans : Transitive M.toFrame.Rel) (r : M.World) : M.mkTransTreeUnravelling r →ₚ M :=
+  PseudoEpimorphism.ofAtomic (Frame.mkTransTreeUnravelling.pMorphism M.toFrame M_trans r) $ by rfl;
+
+protected abbrev root {M : Kripke.Model} {r : M.World} : (M.mkTransTreeUnravelling r).World := Frame.mkTransTreeUnravelling.root
+
+/-
+instance instTree_of_trans_irrefl {M : Model} [DecidableEq M.World] [M.IsFinite] {r : M.World} (F_trans : Transitive M.Rel) (F_irrefl : Irreflexive M.Rel)
+  : Model.IsFiniteTree ((M↾r).mkTransTreeUnravelling  pointGenerate.root) (mkTransTreeUnravelling.root) := by
+  have := @Frame.mkTransTreeUnravelling.instTree_of_trans_irrefl M.toFrame _ _ r F_trans F_irrefl;
+  sorry;
+-/
+
+/-
+instance instIsTree {M : Model} [DecidableEq M.World] [M.IsFinite] {r : M.World} (M_trans : Transitive M.Rel) (M_irrefl : Irreflexive M.Rel)
+  : (M.mkTransTreeUnravelling r).IsFiniteTree (mkTransTreeUnravelling.root) where
+  frame_isFiniteTree := @Frame.mkTransTreeUnravelling.instIsTree M.toFrame _ _ r M_trans M_irrefl;
+-/
+
+protected lemma modal_equivalence_at_root (M : Kripke.Model) (M_trans : Transitive M.toFrame.Rel) (r : M.World)
+  : ModalEquivalent (M₁ := M.mkTransTreeUnravelling r) (M₂ := M) (mkTransTreeUnravelling.root) r
+  := Model.PseudoEpimorphism.modal_equivalence (Model.mkTransTreeUnravelling.pMorphism M M_trans r) (mkTransTreeUnravelling.root)
+
+end Model.mkTransTreeUnravelling
+
 
 
 end TreeUnravelling
